src/tls/IV.fst
@@ -3,12 +3,8 @@ module IV
 open Mem
 open Pkg 
 
-let sample (len:UInt32.t): ST (Bytes.lbytes32 len)
-    (requires fun h0 -> True)
-    (ensures fun h0 r h1 -> h0 == h1)
-  = assume false; Random.sample32 len
 
-
+ 
 /// A sample functionality for fresh, public initialization vectors,
 /// with the length of the byte vector as a basic agility
 /// parameter. We use this functionality e.g. for generating the
@@ -24,8 +20,10 @@ type rawlen (#ip:ipkg) (len_of_i:ip.t -> keylen) (i:ip.t) = len:keylen {len == l
 
 type raw (ip:ipkg) (len_of_i:ip.t -> keylen) (i:ip.t{ip.registered i}) = Bytes.lbytes32 (len_of_i i)
 
+noextract 
 let shared_footprint_raw (ip:ipkg) (len_of_i:ip.t -> keylen): rset = Set.empty
 
+noextract 
 let footprint_raw (ip:ipkg) (len_of_i:ip.t -> keylen)
   (#i:ip.t {ip.registered i}) (k:raw ip len_of_i i)
   : GTot (s:rset{s `Set.disjoint` shared_footprint_raw ip len_of_i})
@@ -35,12 +33,13 @@ let footprint_raw (ip:ipkg) (len_of_i:ip.t -> keylen)
   Set.lemma_equal_elim (fp `Set.intersect` sfp) Set.empty;
   fp
 
+noextract 
 let create_raw (ip:ipkg) (len_of_i:ip.t -> keylen)
   (i:ip.t{ip.registered i}) (len:keylen {len = len_of_i i}):
   ST (raw ip len_of_i i)
   (requires fun h0 -> model)
   (ensures fun h0 p h1 -> modifies_none h0 h1)
-  = sample len
+  = Random.sample32 len
 
 let coerceT_raw (ip:ipkg) (len_of_i:ip.t -> keylen)
   (i: ip.t {ip.registered i /\ (idealRaw ==> ~(ip.honest i))})
@@ -55,6 +54,7 @@ let coerce_raw (ip: ipkg) (len_of_i: ip.t -> keylen)
   (ensures fun h0 k h1 -> k == coerceT_raw ip len_of_i i len r /\ modifies_none h0 h1)
   = r
 
+inline_for_extraction
 let local_raw_pkg (ip:ipkg) (len_of_i:ip.t -> keylen) : local_pkg ip =
   LocalPkg
     (raw ip len_of_i)
@@ -71,8 +71,27 @@ let local_raw_pkg (ip:ipkg) (len_of_i:ip.t -> keylen) : local_pkg ip =
     (coerceT_raw ip len_of_i)
     (coerce_raw ip len_of_i)
 
+inline_for_extraction
 let rp (ip:ipkg) (len_of_i:ip.t -> keylen): ST (pkg ip)
   (requires fun h0 -> True)
   (ensures fun h0 p h1 -> modifies_one tls_define_region h0 h1 /\ p.package_invariant h1)
   =
   memoization_ST (local_raw_pkg ip len_of_i)
+
+(*
+// does this extract? 18-09-24 no
+
+let test() : ST unit 
+  (requires fun h0 -> True)
+  (ensures fun h0 _ h1 -> True)
+  = 
+  let id = n:nat {n < 256} in 
+  let ip : ipkg = Pkg.Idx id (fun _ -> True) (fun _ -> True) (fun _ -> true) in
+  let len_of_i (i:id): keylen = Integers.u i in 
+  let p = local_raw_pkg ip len_of_i in 
+  // let table = mem_alloc (key ip) in 
+  // let q = Pkg.memoization p table in 
+  assume False; 
+  let v0 = p.coerce 12 in  
+  ()
+*)  
